cfrontend/ClightBigstep.v
@@ -259,7 +259,7 @@ Inductive bigstep_program_terminates (p: program): trace -> int -> Prop :=
       Genv.find_funct_ptr ge b = Some f ->
       type_of_fundef f = Tfunction Tnil type_int32s cc_default ->
       Mem.alloc m0 0 0 = (m01,b1) ->
-      Mem.record_stack_blocks m01 (make_singleton_frame_adt b1 0 0) m02 ->
+      Mem.record_stack_blocks false m01 (make_singleton_frame_adt b1 0 0) m02 ->
       eval_funcall ge function_entry m02 f nil t m1 (Vint r) (fn_stack_requirements (prog_main p))->
       bigstep_program_terminates p t r.
 
@@ -271,7 +271,7 @@ Inductive bigstep_program_diverges (p: program): traceinf -> Prop :=
       Genv.find_funct_ptr ge b = Some f ->
       type_of_fundef f = Tfunction Tnil type_int32s cc_default ->
       Mem.alloc m0 0 0 = (m01,b1) ->
-      Mem.record_stack_blocks m01 (make_singleton_frame_adt b1 0 0) m02 ->
+      Mem.record_stack_blocks false m01 (make_singleton_frame_adt b1 0 0) m02 ->
       evalinf_funcall ge function_entry m02 f nil t (fn_stack_requirements (prog_main p)) ->
       bigstep_program_diverges p t.
 
