common/Memtype.v
@@ -184,7 +184,11 @@ that we now axiomatize. *)
 
  (* Stack ADT and methods *)
  stack_adt: mem -> stack_adt;
- record_stack_blocks: mem -> frame_adt -> mem -> Prop;
+ (* [record_stack_blocks tail m1 f m2] records frame information [f] from memory
+ [m1] to [m2]. [tail] is a boolean indicating whether the new frame corresponds
+ to a tailcall ([true]) or not ([false]). *)
+ record_stack_blocks: bool -> mem -> frame_adt -> mem -> Prop;
+ (* record_stack_blocks_tailcall: mem -> frame_adt -> mem -> Prop; *)
  push_frame: mem -> frame_info -> list (memory_chunk * ptrofs * val) -> option (mem*block);
  record_stack_blocks_none: forall (m: mem) (bl : list (block * frame_info)) (sz: Z),
                            Forall
@@ -1394,10 +1398,9 @@ Class MemoryModel mem `{memory_model_ops: MemoryModelOps mem}
    f b = Some (b2, delta') ->
    perm m1 b ofs k p ->
    lo + delta <= ofs + delta' < hi + delta -> False) ->
-  (* (forall (f2 : frame_adt) (fi : frame_info), *)
-  (*     ~ In f2 (stack_adt m2) -> *)
-  (*     In (b2,fi) (frame_adt_blocks f2) -> *)
-  (*     forall (o : Z) (k : perm_kind) (pp : permission), perm m1' b1 o k pp -> inject_perm_condition pp -> frame_public fi (o + delta)) -> *)
+  (forall (fi : frame_info),
+      in_stack' (stack_adt m2) (b2,fi) ->
+      forall (o : Z) (k : perm_kind) (pp : permission), perm m1' b1 o k pp -> inject_perm_condition pp -> frame_public fi (o + delta)) ->
   exists f',
      inject f' g m1' m2
   /\ inject_incr f f'
@@ -1660,7 +1663,7 @@ for [unchanged_on]. *)
      (INJ: inject j g m1 m2)
      (FAP: frame_at_pos (stack_adt m2) 0 f2)
      (FI: tframe_inject j (f1,nil) f2)
-     (RSB: record_stack_blocks m1 f1 m1'),
+     (RSB: record_stack_blocks false m1 f1 m1'),
      inject j (fun n : nat => if Nat.eq_dec n 0 then Some O else g (Init.Nat.pred n)) m1' m2;
 
  record_stack_blocks_inject_parallel {injperm: InjectPerm}:
@@ -1673,16 +1676,16 @@ for [unchanged_on]. *)
               forall o k p, perm m2 b o k p -> 0 <= o < frame_size fi) ->
      (forall (b1 b2 : block) (delta : Z), j b1 = Some (b2, delta) -> in_frame fi1 b1 <-> in_frame fi2 b2) ->
      frame_adt_size fi1 = frame_adt_size fi2 ->
-     record_stack_blocks m1 fi1 m1' ->
+     record_stack_blocks false m1 fi1 m1' ->
      exists m2',
-       record_stack_blocks m2 fi2 m2' /\
+       record_stack_blocks false  m2 fi2 m2' /\
        inject j (fun n => if Nat.eq_dec n 0 then Some O else option_map S (g (pred n))) m1' m2';
 
 
  record_stack_blocks_extends {injperm: InjectPerm}:
     forall m1 m2 m1' fi,
       extends m1 m2 ->
-      record_stack_blocks m1 fi m1' ->
+      record_stack_blocks false m1 fi m1' ->
       (forall b, in_frame fi b -> ~ in_stack ( (stack_adt m2)) b ) ->
       Forall
         (fun b : block * frame_info =>
@@ -1690,22 +1693,28 @@ for [unchanged_on]. *)
              perm m2 (fst b) o k p -> 0 <= o < frame_size (snd b)) 
         (frame_adt_blocks fi) ->
       exists m2',
-        record_stack_blocks m2 fi m2' /\
+        record_stack_blocks false m2 fi m2' /\
         extends m1' m2';
 
  record_stack_blocks_mem_unchanged:
-   forall bfi,
-     mem_unchanged (fun m1 m2 => record_stack_blocks m1 bfi m2);
+   forall bfi tc,
+     mem_unchanged (fun m1 m2 => record_stack_blocks tc m1 bfi m2);
 
  record_stack_blocks_stack_adt:
    forall m fi m',
-     record_stack_blocks m fi m' ->
+     record_stack_blocks false m fi m' ->
      stack_adt m' = (fi,nil) :: stack_adt m;
+
+ record_stack_blocks_tailcall_stack_adt:
+   forall m fi m' f s,
+     record_stack_blocks true m fi m' ->
+     stack_adt m = f::s ->
+     stack_adt m' = (acons fi f) :: s;
 
  record_stack_blocks_inject_neutral {injperm: InjectPerm}:
    forall thr m fi m',
      inject_neutral thr m ->
-     record_stack_blocks m fi m' ->
+     record_stack_blocks false m fi m' ->
      Forall (fun b => Plt b thr) (map fst (frame_adt_blocks fi)) ->
      inject_neutral thr m';
 
@@ -1842,37 +1851,35 @@ for [unchanged_on]. *)
    forall m1 b fi l m4 fa,
      push_frame m1 fi l = Some (m4,b) ->
      frame_adt_blocks fa = (b,fi)::nil ->
-     frame_adt_size fa = frame_size fi ->
+     frame_adt_size fa = Z.max 0 (frame_size fi) ->
      exists m2,
        alloc m1 0 (frame_size fi) = (m2, b) /\
        exists m3,
          do_stores m2 (store_spec_of_ofs_spec b l) = Some m3 /\
-         record_stack_blocks m3 fa m4;
+         record_stack_blocks false m3 fa m4;
 
  alloc_record_push_frame:
    forall m1 m2 b fi l m3 m4 fa,
      frame_adt_blocks fa = (b,fi)::nil ->
-     frame_adt_size fa = frame_size fi ->
+     frame_adt_size fa = Z.max 0 (frame_size fi) ->
      alloc m1 0 (frame_size fi) = (m2, b) ->
      do_stores m2 (store_spec_of_ofs_spec b l) = Some m3 ->
-     record_stack_blocks m3 fa m4 ->
+     record_stack_blocks false m3 fa m4 ->
      push_frame m1 fi l = Some (m4,b);
 
  record_stack_blocks_none_correct:
    forall m (bl: list (block * frame_info)) sz m',
      (exists pf, record_stack_blocks_none m bl sz pf = Some m') <->
-     (exists fa, record_stack_blocks m fa m' /\ frame_adt_blocks fa = bl /\ frame_adt_size fa = sz);
+     (exists fa, record_stack_blocks false m fa m' /\ frame_adt_blocks fa = bl /\ frame_adt_size fa = Z.max 0 sz);
 
  record_stack_block_inject_left_zero {injperm: InjectPerm}:
     forall m1 m1' m2 j g f1 f2
       (INJ: inject j g m1 m2)
       (FAP: frame_at_pos (stack_adt m2) O f2)
       (FI: tframe_inject j (f1,nil) f2)
-      (SZ2: Forall (fun f => 0 = frame_adt_size (ahd f))%Z (stack_adt m2)) 
-      (RSB: record_stack_blocks m1 f1 m1'),
+      (SZ2: Forall (fun f => Forall (fun f =>0 = frame_adt_size f) (to_list f))%Z (stack_adt m2)) 
+      (RSB: record_stack_blocks false m1 f1 m1'),
       inject j (fun n : nat => if Nat.eq_dec n O then Some O else g (pred n)) m1' m2;
-
-
 
  unrecord_stack_block_inject_left_zero {injperm: InjectPerm}:
     forall (m1 m1' m2 : mem) (j : meminj) g,
@@ -1901,7 +1908,7 @@ for [unchanged_on]. *)
         (frame_adt_blocks f) ->
       (size_stack (stack_adt m1) + align (frame_adt_size f) 8 < stack_limit)%Z ->
       exists m2,
-        record_stack_blocks m1 f m2;
+        record_stack_blocks false m1 f m2;
 
  (* record_stack_block_right {injperm: InjectPerm}: *)
  (*   forall j g m1 m2 m2' f, *)
@@ -1912,9 +1919,9 @@ for [unchanged_on]. *)
  (*     inject j (fun n => option_map S (g n)) m1 m2'; *)
 
  record_stack_block_det:
-   forall m f m1 m2,
-     record_stack_blocks m f m1 ->
-     record_stack_blocks m f m2 ->
+   forall m f m1 m2 tc,
+     record_stack_blocks tc m f m1 ->
+     record_stack_blocks tc m f m2 ->
      m1 = m2;
 
  extends_same_length_stack:
@@ -1964,9 +1971,9 @@ record_stack_block_inject_flat {injperm: InjectPerm}:
          forall (o : Z) (k : perm_kind) (p : permission), perm m2 b o k p -> (0 <= o < frame_size fi)%Z)
      (EQINF: forall (b1 b2 : block) (delta : Z), j b1 = Some (b2, delta) -> in_frame f1 b1 <-> in_frame f2 b2)
      (EQsz: frame_adt_size f1 = frame_adt_size f2)
-     (RSB: record_stack_blocks m1 f1 m1'),
+     (RSB: record_stack_blocks false m1 f1 m1'),
      exists m2',
-       record_stack_blocks m2 f2 m2' /\
+       record_stack_blocks false m2 f2 m2' /\
        inject j (flat_frameinj (length (Mem.stack_adt m1'))) m1' m2' /\
        (length (Mem.stack_adt m1) = length (Mem.stack_adt m2) ->
         length (Mem.stack_adt m1') = length (Mem.stack_adt m2'));
@@ -1985,22 +1992,24 @@ mem_inject_tailcall_inlined {injperm: InjectPerm}:
     forall F g m m'0 stk szstk
       (INJ: inject F g m m'0)
       m' (FREE: Mem.free m stk 0 szstk = Some m') 
-      m'' (USB: Mem.unrecord_stack_block m' = Some m'' )
-      m'1 stk0 szstk0 (ALLOC: Mem.alloc m'' 0 szstk0 = (m'1, stk0))
-      stkreq m''0 (RSB: Mem.record_stack_blocks m'1 (make_singleton_frame_adt stk0 szstk0 stkreq) m''0)
+      (* m'' (USB: Mem.unrecord_stack_block m' = Some m'' ) *)
+      m'1 stk0 szstk0 (ALLOC: Mem.alloc m' 0 szstk0 = (m'1, stk0))
+      stkreq m''0 (RSB: Mem.record_stack_blocks true m'1 (make_singleton_frame_adt stk0 szstk0 stkreq) m''0)
       sp' delta (Fstk: F stk = Some (sp', delta))
       delta0
       (LE: (delta <= delta0)%Z)
       (PERMinjstk0: forall o, (0 <= o < szstk0)%Z -> Mem.perm m'0 sp' (o + delta0) Cur Freeable)
       (DIV: Mem.inj_offset_aligned delta0 szstk0)
       (G0 : g O = Some O)
-      (STACKTOP: get_stack_top_blocks (stack_adt m) = stk::nil)
+      f1 s1
+      (STKeq: stack_adt m = f1::s1)
+      (STACKTOP: get_frame_blocks (ahd f1) = stk::nil)
       (PERMstk: forall o k p, perm m stk o k p -> (0 <= o < szstk)%Z)
       sz1 sz2
       (STACKTOP':  exists r rt, stack_adt m'0 = (make_singleton_frame_adt sp' sz1 sz2,rt) :: r)
       (RNG: forall o : Z, (0 <= o < szstk0)%Z -> (0 <= o + delta0 < sz1)%Z)
       (JBstack: forall b, in_stack (stack_adt m) b -> exists b' delta, F b = Some (b', delta))
-      (SIZE: (sz2 <= stkreq)%Z)
+      (* (SIZE: (sz2 <= stkreq)%Z) *)
       (PERMsp': forall b d o p,
           F b = Some (sp', d) -> b <> stk ->
           perm m b o Max p ->
@@ -2009,6 +2018,12 @@ mem_inject_tailcall_inlined {injperm: InjectPerm}:
     ,
       let F' := fun b => if peq b stk0 then Some (sp', delta0) else F b in
       inject F' g m''0 m'0;
+
+record_stack_blocks_tailcall_original_stack:
+  forall m1 f m2,
+    record_stack_blocks true m1 f m2 ->
+    exists f r,
+      stack_adt m1 = f::r;
 
 }.
 
@@ -2140,16 +2155,16 @@ Proof.
 Qed.
 
 Lemma record_stack_block_unchanged_on:
-  forall m bfi m' (P: block -> Z -> Prop),
-    record_stack_blocks m bfi m' ->
+  forall m bfi m' tc (P: block -> Z -> Prop),
+    record_stack_blocks tc m bfi m' ->
     strong_unchanged_on P m m'.
 Proof.
   intros; eapply record_stack_blocks_mem_unchanged; eauto.
 Qed.
 
 Lemma record_stack_block_perm:
-  forall m bfi m',
-    record_stack_blocks m bfi m' ->
+  forall m bfi m' tc,
+    record_stack_blocks tc m bfi m' ->
     forall b' o k p,
       perm m' b' o k p ->
       perm m b' o k p.
@@ -2159,8 +2174,8 @@ Proof.
 Qed.
 
 Lemma record_stack_block_perm'
-  : forall m m' bofi,
-    record_stack_blocks m bofi m' ->
+  : forall m m' bofi tc,
+    record_stack_blocks tc m bofi m' ->
     forall (b' : block) (o : Z) (k : perm_kind) (p : permission),
       perm m b' o k p -> perm m' b' o k p.
 Proof.
@@ -2169,8 +2184,8 @@ Proof.
 Qed.
 
 Lemma record_stack_block_valid:
-  forall m bf m',
-    record_stack_blocks m bf m' ->
+  forall m bf m' tc,
+    record_stack_blocks tc m bf m' ->
     forall b', valid_block m b' -> valid_block m' b'.
 Proof.
   unfold valid_block; intros.
@@ -2179,8 +2194,8 @@ Proof.
 Qed.
 
 Lemma record_stack_block_nextblock:
-  forall m bf m',
-    record_stack_blocks m bf m' ->
+  forall m bf m' tc,
+    record_stack_blocks tc m bf m' ->
     nextblock m' = nextblock m.
 Proof.
   intros.
@@ -2189,16 +2204,21 @@ Proof.
 Qed.
 
 Lemma record_stack_block_is_stack_top:
-  forall m b fi m',
-    record_stack_blocks m fi m' ->
+  forall m b fi m' tc,
+    record_stack_blocks tc m fi m' ->
     in_frame fi b ->
     is_stack_top (stack_adt m') b.
 Proof.
   unfold is_stack_top, get_stack_top_blocks.
   intros.
-  erewrite record_stack_blocks_stack_adt; eauto.
-  unfold get_frames_blocks. simpl.
-  rewrite in_app; left. auto.
+  destruct tc.
+  - edestruct (record_stack_blocks_tailcall_original_stack _ _ _ H) as (f & r & EQ).
+    erewrite record_stack_blocks_tailcall_stack_adt; eauto.
+    unfold get_frames_blocks. simpl.
+    rewrite in_app; left. auto.
+  - erewrite record_stack_blocks_stack_adt; eauto.
+    unfold get_frames_blocks. simpl.
+    rewrite in_app; left. auto.
 Qed.
 
 Lemma unrecord_stack_block_unchanged_on:
